Makefile
@@ -1,10 +1,13 @@
 # ===================================================================
-# Copyright 2022 ZhengPu Shi
-#  This file is part of VFCS. It is distributed under the MIT
+# Copyright 2024 ZhengPu Shi
+#  This file is part of GenProg. It is distributed under the MIT
 #  "expat license". You should have recieved a LICENSE file with it.
 # ===================================================================
 
 COQMAKEFILE ?= Makefile.coq
+
+MY_HTML_ROOT = doc/GenProg
+MY_HTML_ROOT_WITH_VERSION = $(MY_HTML_ROOT)/v1.0
 
 HTML_EXTRA_DIR = html-extra
 COQDOCFLAGS ?= \
@@ -13,7 +16,7 @@ COQDOCFLAGS ?= \
   --no-lib-name \
   --with-header $(HTML_EXTRA_DIR)/header.html \
   --with-footer $(HTML_EXTRA_DIR)/footer.html \
-  --parse-comments
+  # --parse-comments
 export COQDOCFLAGS
 
 all: $(COQMAKEFILE)
@@ -22,6 +25,17 @@ all: $(COQMAKEFILE)
 $(COQMAKEFILE): _CoqProject
 	$(COQBIN)coq_makefile -f $^ -o $@
 
+html: $(COQMAKEFILE)
+	rm -rf html/
+	rm -rf $(MY_HTML_ROOT_WITH_VERSION)
+	mkdir -p $(MY_HTML_ROOT)
+	$(MAKE) -f $^ $@
+	mv html $(MY_HTML_ROOT_WITH_VERSION)
+	cp $(HTML_EXTRA_DIR)/index.html $(MY_HTML_ROOT)/
+	cp $(HTML_EXTRA_DIR)/header.html $(MY_HTML_ROOT_WITH_VERSION)/
+	cp $(HTML_EXTRA_DIR)/footer.html $(MY_HTML_ROOT_WITH_VERSION)/
+	cp $(HTML_EXTRA_DIR)/resources $(MY_HTML_ROOT_WITH_VERSION)/ -R
+
 clean: $(COQMAKEFILE)
 	$(MAKE) -f $^ cleanall
 
@@ -29,15 +43,4 @@ cleanall: $(COQMAKEFILE)
 	$(MAKE) -f $^ cleanall
 	$(RM) $^ $^.conf
 
-html: $(COQMAKEFILE)
-	$(MAKE) -f $^ $@
-	cp $(HTML_EXTRA_DIR)/* html/ -R
-
-install: $(COQMAKEFILE)
-	$(MAKE) -f $^ install
-
-uninstall: $(COQMAKEFILE)
-	$(MAKE) -f $^ uninstall
-
-
-.PHONY: all clean cleanall html install uninstall
+.PHONY: all clean cleanall html
